src/crypto/poly1305/x64/X64.Poly1305.Math_i.fsti
@@ -4,6 +4,13 @@ open FStar.Mul
 open X64.Machine_s   // needed for nat64
 open X64.Vale.Decls  // needed for shift_right64, logand64
 
+let lowerUpper128 (l:nat64) (u:nat64) : nat128 =
+    0x10000000000000000 `op_Multiply` u + l
+
+let lowerUpper192 (l:nat128) (u:nat64) : int =
+    0x100000000000000000000000000000000 `op_Multiply` u + l
+
+
 // p used to be a refinement to p > 0 and r1 a nat.
 // There are some assumptions here, which will either go away when the library switches to ints everywhere (for division too)
 // or when we switch to nats (which is doable right away)
@@ -58,3 +65,40 @@ val lemma_mul_strict_upper_bound : x:nat -> x_bound:int -> y:nat -> y_bound:int 
     y < y_bound)
   (ensures x * y < x_bound * y_bound)
     
+val lemma_bytes_shift_power2 : y:nat64 -> Lemma
+  (requires y < 8)
+  (ensures 
+    shift_left64 y 3 < 64 /\
+    shift_left64 y 3 == y * 8 /\
+    pow2 (shift_left64 y 3) == shift_left64 1 (shift_left64 y 3))
+    
+val lemma_bytes_and_mod : x:nat64 -> y:nat64 -> Lemma
+  (requires y < 8)
+  (ensures 
+    shift_left64 y 3 < 64 /\
+    (let z = shift_left64 1 (shift_left64 y 3) in
+     z <> 0 /\ logand64 x z-1 == x % z))
+
+val lemma_mod_power2_lo : x0:nat64 -> x1:nat64 -> y:int -> z:int -> Lemma
+  (requires 
+    0 <= y /\ y < 8 /\
+    z == pow2 (y * 8))
+  (ensures 
+    z > 0 /\
+    0 <= x0 % z /\ 
+    x0 % z < 0x10000000000000000 /\
+    (lowerUpper128 x0 x1) % z == (lowerUpper128 (x0 % z) 0))
+    
+val lemma_power2_add64 : n:nat -> Lemma
+  (requires True)
+  (ensures pow2(64 + n) == 0x10000000000000000 * pow2(n))
+
+val lemma_mod_hi : x0:nat64 -> x1:nat64 -> z:nat64 -> Lemma
+  (requires z <> 0)
+  (ensures
+    lowerUpper128 0 z <> 0 /\
+    (lowerUpper128 x0 x1) % (lowerUpper128 0 z) == lowerUpper128 x0 (x1 % z))
+
+val lemma_poly_demod : p:int -> h:int -> x:int -> r:int -> Lemma
+  (requires p > 0)
+  (ensures p > 0 /\ ((h % p + x) * r) % p == ((h + x) * r) % p)
